Set the following variables:
\begin{align*}
    S_p &= \frac{S}{N}\\
    I_p &= \frac{I}{N}\\
    R_p &= \frac{R}{N}\\
    N_p &= \frac{N}{N} = 1
\end{align*}
Then substitute these variables into the equations (1)
\begin{align}
  \frac{dS_p}{dt} &= \mu N_p -\frac{\beta}{N_p} S_p I_p - \mu S_p\\
                  &= \mu 1 -\frac{\beta}{1} S_p I_p - \mu S_p\\
                  &= \frac{1}{N}(\mu -\beta SI - \mu S)\\
                  &= \frac{1}{N} \frac{dS}{dt}\\
  \vspace{8pt}
  \frac{dI_p}{dt} &= \frac{\beta}{N_p} S_p I_p - \gamma I_p - \mu I_p\\
                  &= \frac{\beta}{1} S_p I_p - \gamma I_p - \mu I_p\\
                  &= \frac{1}{N} (\beta SI - \gamma I - \mu I)\\
                  &= \frac{1}{N} \frac{dI}{dt}\\
  \vspace{8pt}
  \frac{dR_p}{dt} &= \gamma I_p - \mu R_p\\
                  &= \frac{1}{N} (\gamma I - \mu R)\\
                  &= \frac{1}{N} \frac{dR}{dt}
\end{align}
From this it is clear that the proportional equations for $\frac{dS_p}{dt},\frac{dI_p}{dt},\frac{dR_p}{dt}$ are equivalent to the original equations (1), just scaled by a constant factor of $\frac{1}{N}$, and thus will retain the same dynamical behaviour.
