The EE is $(\hat{S},\hat{I}) = (\frac{1}{{\mathcal R_0}},\eps(1-\frac{1}{{\mathcal R_0}})$.
Consider the Lyapunov function with ${\mathcal O} = \{(S,I) | 0\leq S,I \leq 1\ and\ S+I = 1\} $
\begin{align}
    L(S,I) &= S - \frac{1}{{\mathcal R_0}}log(S) + I - \eps(1-\frac{1}{{\mathcal R_0}})log(I)\nonumber\\
           &= S - \frac{1}{{\mathcal R_0}}log(S) + I - \eps log(I) -(\frac{\eps}{{\mathcal R_0}})log(I)\nonumber\\
           &= S - \frac{1}{{\mathcal R_0}}log(S) + I + \eps log(I) (\frac{1}{{\mathcal R_0}}-1)\label{lup}\\
    0 \leq S,I \leq 1 &\implies log(S), log(I) < 0 \implies \nonumber\\
    0   &< S - \frac{1}{{\mathcal R_0}}log(S) + I + \eps log(I) (\frac{1}{{\mathcal R_0}}-1)\label{pos}
\end{align}
Thus \ref{pos} shows that \ref{lup} is positive on $[0,1]$, the the function is postive definite on $[0,1]$.
\begin{align}
    L(\hat{S},\hat{I})  &= \hat{S} - \hat{S}log(\hat{S}) + \hat{I}\\
    &= \hat{S} - \frac{1}{{\mathcal R_0}}log(\frac{1}{{\mathcal R_0}}) + I - \eps(1-\frac{1}{{\mathcal R_0}})log(I)\label{lupeq}\\
\end{align}
From Lyapunov's theorem, a function $L(X)$ satisfies $L(X) > L(X_*) \forall\ X \in {\mathcal O} \setminus \{X_*\}$ where $X_* = (\hat{S},\hat{I})$, and using the same set ${\mathcal O}$ as defined earilier.
\begin{align}
    L(S,I) &> L(\hat{S},\hat{I})\nonumber\\
    S - \hat{S}log(S) +I - \hat{I}log(I) &> \hat{S} - \hat{S}log(\hat{S}) +\hat{I} - \hat{I}log(\hat{I})\nonumber
\end{align}
\begin{align}
    \frac{\partial L}{\partial S} &= 1 - \frac{\hat{S}}{S}\nonumber\\
    \frac{\partial L}{\partial S} &= 1 - \frac{\hat{S}}{S} = 0 \implies S = \hat{S}\nonumber\\
    \frac{\partial L}{\partial I} &= 1 - \frac{\hat{I}}{I}\nonumber\\
    \frac{\partial L}{\partial I} &= 1 - \frac{\hat{I}}{I} = 0 \implies I = \hat{I}\nonumber
\end{align}
The functions $log(S), log(I)$ increase monotonically with respect to $\hat{S},\hat{I}$. Both partial derivatives $\frac{\partial L}{\partial S}, \frac{\partial L}{\partial I}$ as well, the by \ref{mono1}, \ref{mono2} show that $(\hat{S},\hat{I}$ must be the global minimum of $L(S,I)$ on $[0,1]$.\\
Further
\begin{align}
    \frac{\partial^2 L}{\partial S^2} &= \hat{S}S^{-2} \textrm{at} \hat{S} = \frac{\hat{S}}{\hat{S}^2} = \frac{1}{\hat{S}}\nonumber\\
    \frac{\partial^2 L}{\partial I^2} &= \hat{I}I^{-2} \textrm{at} \hat{I} = \frac{\hat{I}}{\hat{I}^2} = \frac{1}{\hat{I}}\nonumber\\
\end{align}
are non-negative at the minimum point $(\hat{S},\hat{I})$, thus $L(S,I) > L(\hat{S},\hat{I}) \forall\ (S,I) \in {\mathcal O} \setminus \{(\hat{S},\hat{I})\}$.
From \ref{sp}, \ref{ip}
\begin{align}
    0 &= \beta \hat{S} \hat{I} - \gamma \hat{I} - \mu \hat{I} \implies \beta \hat{S} \hat{I} = \gamma \hat{I} + \mu \hat{I}\nonumber\\
    0 &= \mu - \beta \hat{S} \hat{I} + \mu \hat{S} \implies \beta \hat{S} \hat{I} = \mu - \mu \hat{S}\nonumber\\
    \dot{L} &= (1-\frac{1}{{\mathcal R_0}})(\mu - \beta SI - \mu S) + (1 - \frac{\eps(1 - \frac{1}{{\mathcal R_0}})}{I})(\beta SI - \gamma I \mu I)\nonumber\\
            &= \mu - \mu \hat{S} - \frac{\mu}{{\mathcal R_0}\hat{S}} + \frac{\beta \hat{I}}{{\mathcal R_0}} + \frac{\mu}{{\mathcal R_0}} - \gamma \hat{I} - \mu \hat{I} - \beta \hat{S} \hat{I} + \gamma \hat{I} + \mu \hat{I}\nonumber\\
            &= \mu(2 - S - \frac{1}{{\mathcal R_0} S}) + \frac{\beta I}{{\mathcal R_0}} - \frac{\beta S}{\mathcal R_0}(\eps{\mathcal R_0}-\eps) - I(\gamma+\mu)\nonumber\\
            &= \mu(2 - S - \frac{1}{{\mathcal R_0} S}) + \frac{\beta}{{\mathcal R_0}}(I - S\eps {\mathcal R_0} + S \eps) - I \frac{\mu}{\eps}\nonumber\\
            &= \mu(2 - S - \frac{1}{{\mathcal R_0} S}) + \frac{\mu}{\eps}(I - S\eps {\mathcal R_0} + S \eps) - I \frac{\mu}{\eps}\nonumber\\
            &= \mu(2 - S - \frac{1}{{\mathcal R_0} S}) + \frac{\mu}{\eps}(I - S\eps {\mathcal R_0} + S \eps -I) \nonumber\\
            &= \mu(2 - S - \frac{1}{{\mathcal R_0} S}) + \frac{\mu}{\eps}(-S\eps {\mathcal R_0} + S \eps) \nonumber\\
            &= \mu(2 - S - \frac{1}{{\mathcal R_0} S}) + \mu(-S {\mathcal R_0} + S) \nonumber\\
            &= \mu(2 - S - \frac{1}{{\mathcal R_0} S} -S {\mathcal R_0} + S) \nonumber\\
            &= \mu(2 - \frac{\hat{S}}{S} - \frac{S}{\hat{S}})\nonumber\\
            &= -\mu( \frac{\hat{S}}{S} + \frac{S}{\hat{S}}-2)\nonumber\\
            &= -\mu\frac{\hat{S}}{S}(1- 2\frac{S^2}{\hat{S}^2})\nonumber\\
            &= -\mu\frac{\hat{S}}{S}(1- \frac{S}{\hat{S}})^2\label{fin}
\end{align}

By \ref{fin} $\dot{L}(S,I) \leq 0 \forall\ (S,I) \in (0,1)$ and from earlier $\dot{L}(\hat{S},\hat{I}) = 0$.
Hence $\dot{L}$ is negative definite on $(0,1)$.
Therefore $L(S,I)$ is a strict Lyapunov function for the EE for the biologically relevant states, excluding the DFE, which implies the EE is GAS.
