\begin{proof}
      	\begin{align*}
      		\frac{dI}{dt}                                   &= \beta I(N-I)\\
      		\int\frac{1}{I(N-I)} dI                         &= \int\beta dt\\
      		\frac{1}{N}\int (\frac{1}{I} + \frac{1}{N-1})dI &= \beta t + C\\
      		\frac{1}{N}(ln|I|- ln|N-I|)                     &= \beta t + C\\
      		ln\abs{\frac{I}{N-I}}                           &= N \beta t + NC\\
      		\frac{N-I}{I}                                   &= \pm e^{-NC}e^{-N\beta t}\\	
      	\end{align*}
           	
      	Let $k = \pm e^{-C_2}$\\
      	\begin{align*}
      		\frac{N-I}{I} 	      &= ke^{-N\beta t}\\
      		\frac{N}{I} - 1         &= ke^{-N\beta t}\\
      		\frac{N}{I} 	      &= 1 + ke^{-N\beta t}\\
      		I(t) 			      &= \frac{N}{1 + ke^{-N\beta t}}\\
      	\end{align*}
      	
      	To solve for $k$, let $I(0) = I_0$.\\
      	\begin{align*}
      		I(0) 	&= I_0 = \frac{N}{1 + k}\\ 
      		k 		&= \frac{N - I_0}{I_0}\\
      	\end{align*}
      	
        So the exact solution of the model is
        \begin{equation}
          I(t) =  \frac{N}{1+\frac{N-I_0}{I_0}(e^{-\beta N t})}
        \end{equation}
        
        Since 
        $$\lim_{t\to\infty} e^{-\beta N t} = 0$$
       $$\lim_{t\to\infty} I(t) = \frac{N}{1 +\frac{N-I_0}{I_0}(0)} = N$$
       then every solution that starts in the interval $(0, N)$ converges to the EE. 
      \end{proof}

